proof/correctness/Issues/Normr_Simpl.ec
@@ -1,0 +1,16 @@
+require import Int.
+
+print "`|_|".
+print CoreInt.absz.
+
+op P : int -> bool.
+axiom P2 : P 2.
+
+lemma oops : P `|2|.
+proof.
+(*This does nothing because CoreInt.absz is an op.*)
+rewrite //=.
+move: P2.
+(*Then why does this work?*)
+rewrite //.
+qed.
